Monad transformers preserve ordering

Discretion/Monad/Ordered.lean
@@ -1,9 +1,19 @@
 import Discretion.Order.Discrete
+import Discretion.Nonempty.Set
 import Mathlib.Data.Set.Functor
+import Mathlib.Control.Monad.Writer
 
 instance Disc.instMonad : Monad Disc := Id.instMonad
 
 instance Disc.instLawfulMonad : LawfulMonad Disc := Id.instLawfulMonad
+
+instance WithTop.instMonad : Monad WithTop := (inferInstance : Monad Option)
+
+instance WithTop.instLawfulMonad : LawfulMonad WithTop := (inferInstance : LawfulMonad Option)
+
+instance WithBot.instMonad : Monad WithBot := (inferInstance : Monad Option)
+
+instance WithBot.instLawfulMonad : LawfulMonad WithBot := (inferInstance : LawfulMonad Option)
 
 instance DiscTop.instMonad : Monad DiscTop := (inferInstance : Monad Option)
 
@@ -33,8 +43,14 @@ theorem DiscBot.bind_some {α β} (a : α) (f : α → DiscBot β) : some a >>= 
 @[simp]
 theorem DiscBot.bind_coe {α β} (a : α) (f : α → DiscBot β) : a >>= f = f a := rfl
 
-class OrderedMonad (m : Type u → Type v) [Monad m] [∀α, LE (m α)] where
+class OrderedMonad (m : Type u → Type v) [Bind m] [∀α, LE (m α)] where
   bind_mono {α β} {a a' : m α} {f f' : α → m β} (ha : a ≤ a') (hf : f ≤ f') : a >>= f ≤ a' >>= f'
+
+theorem OrderedMonad.map_mono {m : Type u → Type v}
+  [Monad m] [LawfulMonad m] [∀α, Preorder (m α)] [OrderedMonad m]
+  {α β} (f : α → β) {a a' : m α} (ha : a ≤ a') : f <$> a ≤ f <$> a' := by
+  simp only [map_eq_pure_bind]
+  apply OrderedMonad.bind_mono ha (le_refl _)
 
 instance Disc.instOrderedMonad : OrderedMonad Disc where
   bind_mono ha hf := by cases ha; cases (DiscreteOrder.le_eq _ _ hf); rfl
@@ -53,19 +69,127 @@ instance DiscBot.instOrderedMonad : OrderedMonad DiscBot where
 
 -- TODO: DiscBounded is also an OrderedMonad
 
-class TopMonad (m : Type u → Type v) [Monad m] [∀α, Top (m α)] where
+class TopMonad (m : Type u → Type v) [Bind m] [∀α, Top (m α)] where
   bind_top {α β} (f : α → m β) : ⊤ >>= f = ⊤
 
 instance DiscTop.instTopMonad : TopMonad DiscTop where
   bind_top _ := rfl
 
-class BotMonad (m : Type u → Type v) [Monad m] [∀α, Bot (m α)] where
+class BotMonad (m : Type u → Type v) [Bind m] [∀α, Bot (m α)] where
   bind_bot {α β} (f : α → m β) : ⊥ >>= f = ⊥
 
 instance DiscBot.instBotMonad : BotMonad DiscBot where
   bind_bot _ := rfl
 
 -- TODO: DiscBounded is a TopMonad and a BotMonad
+
+abbrev DiscT (m : Type u → Type v) (α : Type u) := Disc (m α)
+
+instance DiscT.instMonad (m : Type u → Type v) [Hm : Monad m] : Monad (DiscT m) := Hm
+
+instance DiscT.instLawfulMonad (m : Type u → Type v) [Monad m] [Hm : LawfulMonad m]
+  : LawfulMonad (DiscT m) := Hm
+
+instance DiscT.instOrderedMonad (m : Type u → Type v) [Monad m] : OrderedMonad (DiscT m) where
+  bind_mono ha hf := by cases ha; cases discrete_order hf; rfl
+
+instance ReaderT.instLE (m : Type u → Type v) [∀α, LE (m α)] (ρ : Type u) : LE (ReaderT ρ m α)
+  := (inferInstance : LE (ρ → m α))
+
+instance ReaderT.instPreorder (m : Type u → Type v) [∀α, Preorder (m α)] (ρ : Type u)
+  : Preorder (ReaderT ρ m α) := (inferInstance : Preorder (ρ → m α))
+
+instance ReaderT.instPartialOrder (m : Type u → Type v) [∀α, PartialOrder (m α)] (ρ : Type u)
+  : PartialOrder (ReaderT ρ m α) := (inferInstance : PartialOrder (ρ → m α))
+
+instance ReaderT.instOrderedMonad (m : Type u → Type v) [Monad m] [∀α, LE (m α)] [OrderedMonad m]
+  (ρ) : OrderedMonad (ReaderT ρ m) where
+  bind_mono ha hf := by
+    intro r
+    simp only [bind, ReaderT.bind]
+    apply OrderedMonad.bind_mono
+    apply ha
+    intro a
+    apply hf
+
+instance WriterT.instLE (ω) (m : Type u → Type v) (α) [∀α, LE (m α)] : LE (WriterT ω m α)
+  := (inferInstance : LE (m (α × ω)))
+
+instance WriterT.instPreorder (ω) (m : Type u → Type v) [∀α, Preorder (m α)] (α)
+  : Preorder (WriterT ω m α)
+  := (inferInstance : Preorder (m (α × ω)))
+
+instance WriterT.instPartialOrder (ω) (m : Type u → Type v) [∀α, PartialOrder (m α)] (α)
+  : PartialOrder (WriterT ω m α)
+  := (inferInstance : PartialOrder (m (α × ω)))
+
+instance WriterT.instOrderedMonad (ω) (m : Type u → Type v)
+  [Monad m] [LawfulMonad m] [∀α, Preorder (m α)] [OrderedMonad m] [Monoid ω]
+  : OrderedMonad (WriterT ω m) where
+  bind_mono ha hf := by
+    apply OrderedMonad.bind_mono (m := m) ha
+    intro x
+    apply OrderedMonad.map_mono
+    apply hf
+
+instance StateT.instLE (σ) (m : Type u → Type v) (α) [∀α, LE (m α)] : LE (StateT σ m α)
+  := (inferInstance : LE (σ → m (α × σ)))
+
+instance StateT.instPreorder (σ) (m : Type u → Type v) [∀α, Preorder (m α)] (α)
+  : Preorder (StateT σ m α)
+  := (inferInstance : Preorder (σ → m (α × σ)))
+
+instance StateT.instPartialOrder (σ) (m : Type u → Type v) [∀α, PartialOrder (m α)] (α)
+  : PartialOrder (StateT σ m α)
+  := (inferInstance : PartialOrder (σ → m (α × σ)))
+
+instance StateT.instOrderedMonad (σ) (m : Type u → Type v)
+  [Monad m] [LawfulMonad m] [∀α, Preorder (m α)] [OrderedMonad m] : OrderedMonad (StateT σ m) where
+  bind_mono ha hf := by
+    intro s
+    simp only [bind, StateT.bind]
+    apply OrderedMonad.bind_mono (m := m)
+    apply ha
+    intro x
+    apply hf
+
+instance ExceptT.instLE (ε) (m : Type u → Type v) (α) [∀α, LE (m α)] : LE (ExceptT ε m α)
+  := (inferInstance : LE (m (Except ε α)))
+
+instance ExceptT.instPreorder (ε) (m : Type u → Type v) [∀α, Preorder (m α)] (α)
+  : Preorder (ExceptT ε m α)
+  := (inferInstance : Preorder (m (Except ε α)))
+
+instance ExceptT.instPartialOrder (ε) (m : Type u → Type v) [∀α, PartialOrder (m α)] (α)
+  : PartialOrder (ExceptT ε m α)
+  := (inferInstance : PartialOrder (m (Except ε α)))
+
+instance ExceptT.instOrderedMonad (ε) (m : Type u → Type v)
+  [Monad m] [LawfulMonad m] [∀α, Preorder (m α)] [OrderedMonad m] : OrderedMonad (ExceptT ε m) where
+  bind_mono ha hf := by
+    apply OrderedMonad.bind_mono (m := m) ha
+    intro x
+    cases x <;>
+    simp only [ExceptT.bindCont, le_refl]
+    apply hf
+
+instance OptionT.instLE (m : Type u → Type v) [∀α, LE (m α)] : LE (OptionT m α)
+  := (inferInstance : LE (m (Option α)))
+
+instance OptionT.instPreorder (m : Type u → Type v) [∀α, Preorder (m α)] : Preorder (OptionT m α)
+  := (inferInstance : Preorder (m (Option α)))
+
+instance OptionT.instPartialOrder (m : Type u → Type v) [∀α, PartialOrder (m α)]
+  : PartialOrder (OptionT m α) := (inferInstance : PartialOrder (m (Option α)))
+
+instance OptionT.instOrderedMonad (m : Type u → Type v)
+  [Monad m] [LawfulMonad m] [∀α, Preorder (m α)] [OrderedMonad m] : OrderedMonad (OptionT m) where
+  bind_mono ha hf := by
+    apply OrderedMonad.bind_mono (m := m) ha
+    intro x
+    cases x <;>
+    simp only [le_refl]
+    apply hf
 
 -- TODO: more interesting:
 -- - the trace monad with an ordered monoid
@@ -84,3 +208,10 @@ instance Set.bot_monad : BotMonad Set where
   bind_bot _ := by simp
 
 -- Note: set is _not_ a `TopMonad`, since not every α → Set β is a covering!
+
+instance NSet.instOrderedMonad : OrderedMonad NSet where
+  bind_mono ha hf := by
+    simp only [LE.le, bind, coe_subset_iff, coe_iUnion, Set.iUnion_coe_set, Set.iUnion_subset_iff]
+    intro a ha' b hb'
+    simp only [Set.mem_iUnion, exists_prop]
+    exact ⟨a, ha ha', hf a hb'⟩
